fstar/treesync/symbolic/MLS.TreeSync.Symbolic.API.GroupManager.fst
@@ -1,62 +1,56 @@
 module MLS.TreeSync.Symbolic.API.GroupManager
 
 open Comparse
+open DY.Core
+open DY.Lib
 open MLS.NetworkTypes
-open ComparseGlue
-open GlobalRuntimeLib
-open LabeledRuntimeAPI
 open MLS.Symbolic
-open MLS.Symbolic.MapSession
 
 (*** Group manager types & invariants ***)
 
-type group_manager_value (bytes:Type0) {|bytes_like bytes|} = {
+[@@ with_bytes dy_bytes]
+type group_manager_key  = {
+  group_id: mls_bytes dy_bytes;
+}
+
+%splice [ps_group_manager_key] (gen_parser (`group_manager_key))
+%splice [ps_group_manager_key_is_well_formed] (gen_is_well_formed_lemma (`group_manager_key))
+
+[@@ with_bytes dy_bytes]
+type group_manager_value  = {
   [@@@ with_parser #bytes ps_nat]
   si_public: nat;
   [@@@ with_parser #bytes ps_nat]
   si_private: nat;
 }
 
-// When upgrading F* from commit 7ae4850a7e24f011a572ab4097fe1045babab48c to commit eb911fc41d5ba730c15f2ac296ffc5ebf7b46560,
-// We get a failure in the `gen_parser` tactic:
-// Goal: (bytes: Type0), (_: Comparse.Bytes.Typeclass.bytes_like bytes), (x: Prims.nat) |- _ : Prims.squash (forall (y: Prims.nat). (| x, y |) == (| x, y |))
-// Comparse.Tactic.GenerateParser.fst(293,8-293,85): (Error 228) user tactic failed: `apply_lemma: Cannot instantiate lemma FStar.Tactics.Logic.fa_intro_lem (with postcondition: Prims.squash (forall (x: Prims.nat). (| (*?u383*) _, (*?u379*) _ |) == (*?u371*) _)) to match goal (Prims.squash (forall (y: Prims.nat). (| x, y |) == (| x, y |)))` (see also FStar.Tactics.Logic.fst(50,4-50,31))
-// It does not happen in interactive mode, only when compiling using `make`.
-// Very difficult to minimize, modifying functions *after* the tactic call would make the error dissappear.
-// I noticed that adding a dummy function before is fixing the problem.
-// Another option would have been to spend hours minimizing, filing an issue in F* and hope it would be fixed, but I don't have that time right now.
-// This is why there is this horrible hack.
-private let __do_not_remove_me__ (bytes:Type0) = ()
-
 %splice [ps_group_manager_value] (gen_parser (`group_manager_value))
 %splice [ps_group_manager_value_is_well_formed] (gen_is_well_formed_lemma (`group_manager_value))
 
-val group_manager_types: map_types dy_bytes
-let group_manager_types = {
-  key = mls_bytes dy_bytes;
-  ps_key = ps_mls_bytes;
-  value = group_manager_value dy_bytes;
-  ps_value = ps_group_manager_value;
+instance group_manager_types: map_types group_manager_key group_manager_value = {
+  tag = "MLS.TreeSync.GroupManager";
+  ps_key_t = ps_group_manager_key;
+  ps_value_t = ps_group_manager_value;
 }
 
-val group_manager_pred: map_predicate group_manager_types
-let group_manager_pred = {
-  pred = (fun gu time (group_id:group_manager_types.key) value ->
-    is_publishable gu time group_id
+val group_manager_pred: {|crypto_invariants|} -> map_predicate group_manager_key group_manager_value #_
+let group_manager_pred #ci = {
+  pred = (fun tr prin state_id key value ->
+    is_publishable tr key.group_id
   );
-  pred_later = (fun gu time0 time1 key value -> ());
-  pred_is_msg = (fun gu time key value -> ());
+  pred_later = (fun tr1 tr2 prin state_id key value -> ());
+  pred_knowable = (fun tr prin state_id key value -> ());
 }
 
-val group_manager_label: string
-let group_manager_label = "MLS.TreeSync.GroupManager"
+val has_group_manager_invariant: protocol_invariants -> prop
+let has_group_manager_invariant invs =
+  has_map_session_invariant invs group_manager_pred
 
-val has_group_manager_invariant: preds -> prop
-let has_group_manager_invariant pr =
-  has_map_session_invariant group_manager_types group_manager_pred group_manager_label pr
+val group_manager_tag_and_invariant: {|crypto_invariants|} -> string & local_bytes_state_predicate
+let group_manager_tag_and_invariant #ci = (group_manager_types.tag, local_state_predicate_to_local_bytes_state_predicate (map_session_invariant group_manager_pred))
 
 (*** Group manager API ***)
 
-let initialize_group_manager = initialize_map group_manager_types group_manager_pred group_manager_label
-let add_new_group_sessions = add_key_value group_manager_types group_manager_pred group_manager_label
-let find_group_sessions = find_value group_manager_types group_manager_pred group_manager_label
+let initialize_group_manager = initialize_map group_manager_key group_manager_value
+let add_new_group_sessions = add_key_value #group_manager_key #group_manager_value
+let find_group_sessions = find_value #group_manager_key #group_manager_value
