fstar/treesync/symbolic/MLS.TreeSync.Symbolic.API.KeyPackageManager.fst
@@ -1,16 +1,17 @@
 module MLS.TreeSync.Symbolic.API.KeyPackageManager
 
 open Comparse
+open DY.Core
+open DY.Lib
 open MLS.TreeSync.NetworkTypes
 open MLS.Bootstrap.NetworkTypes
-open LabeledRuntimeAPI
 open MLS.Symbolic
-open MLS.Symbolic.MapSession
 open MLS.TreeSync.Symbolic.IsWellFormed
 
 (*** KeyPackage manager types & invariants ***)
 
-type key_package_manager_value (bytes:Type0) {|bytes_like bytes|} = {
+[@@ with_bytes dy_bytes]
+type key_package_manager_value = {
   [@@@ with_parser #bytes ps_nat]
   si_private: nat;
 }
@@ -18,32 +19,32 @@ type key_package_manager_value (bytes:Type0) {|bytes_like bytes|} = {
 %splice [ps_key_package_manager_value] (gen_parser (`key_package_manager_value))
 %splice [ps_key_package_manager_value_is_well_formed] (gen_is_well_formed_lemma (`key_package_manager_value))
 
-val key_package_manager_types: treekem_types dy_bytes -> map_types dy_bytes
-let key_package_manager_types tkt = {
-  key = key_package_nt dy_bytes tkt;
-  ps_key = ps_key_package_nt tkt;
-  value = key_package_manager_value dy_bytes;
-  ps_value = ps_key_package_manager_value;
+instance key_package_manager_types (tkt:treekem_types dy_bytes): map_types (key_package_nt dy_bytes tkt) key_package_manager_value = {
+  tag = "MLS.TreeSync.KeyPackageManager";
+  ps_key_t = ps_key_package_nt tkt;
+  ps_value_t = ps_key_package_manager_value;
 }
 
-val key_package_manager_pred: tkt:treekem_types dy_bytes -> map_predicate (key_package_manager_types tkt)
-let key_package_manager_pred tkt = {
-  pred = (fun gu time (key_package:(key_package_manager_types tkt).key) value ->
-    is_well_formed _ (is_publishable gu time) key_package
+val key_package_manager_pred: {|crypto_invariants|} -> tkt:treekem_types dy_bytes -> map_predicate (key_package_nt dy_bytes tkt) key_package_manager_value #_
+let key_package_manager_pred #ci tkt = {
+  pred = (fun tr prin state_id key_package value ->
+    is_well_formed _ (is_publishable tr) key_package
   );
-  pred_later = (fun gu time0 time1 key_package value -> ());
-  pred_is_msg = (fun gu time key_package value -> ());
+  pred_later = (fun tr1 tr2 prin state_id key_package value -> ());
+  pred_knowable = (fun tr prin state_id key_package value ->
+    assert(is_well_formed _ (is_knowable_by (principal_state_label prin state_id) tr) key_package)
+  );
 }
 
-val key_package_manager_label: string
-let key_package_manager_label = "MLS.TreeSync.KeyPackageManager"
+val has_key_package_manager_invariant: treekem_types dy_bytes -> protocol_invariants -> prop
+let has_key_package_manager_invariant tkt invs =
+  has_map_session_invariant invs (key_package_manager_pred tkt)
 
-val has_key_package_manager_invariant: treekem_types dy_bytes -> preds -> prop
-let has_key_package_manager_invariant tkt pr =
-  has_map_session_invariant (key_package_manager_types tkt) (key_package_manager_pred tkt) key_package_manager_label pr
+val key_package_manager_tag_and_invariant: {|crypto_invariants|} -> treekem_types dy_bytes -> string & local_bytes_state_predicate
+let key_package_manager_tag_and_invariant #ci tkt = ((key_package_manager_types tkt).tag, local_state_predicate_to_local_bytes_state_predicate (map_session_invariant (key_package_manager_pred tkt)))
 
 (*** KeyPackage manager API ***)
 
-let initialize_key_package_manager (tkt:treekem_types dy_bytes) = initialize_map (key_package_manager_types tkt) (key_package_manager_pred tkt) key_package_manager_label
-let add_new_key_package_secret_session (tkt:treekem_types dy_bytes) = add_key_value (key_package_manager_types tkt) (key_package_manager_pred tkt) key_package_manager_label
-let find_key_package_secret_session (tkt:treekem_types dy_bytes) = find_value (key_package_manager_types tkt) (key_package_manager_pred tkt) key_package_manager_label
+let initialize_key_package_manager (tkt:treekem_types dy_bytes) = initialize_map (key_package_nt dy_bytes tkt) key_package_manager_value
+let add_new_key_package_secret_session (tkt:treekem_types dy_bytes) = add_key_value #(key_package_nt dy_bytes tkt) #key_package_manager_value
+let find_key_package_secret_session (tkt:treekem_types dy_bytes) = find_value #(key_package_nt dy_bytes tkt) #key_package_manager_value
