fstar/treesync/symbolic/MLS.TreeSync.Symbolic.GlobalUsage.fst
@@ -1,13 +1,11 @@
 module MLS.TreeSync.Symbolic.GlobalUsage
 
-open FStar.Tactics
-open LabeledCryptoAPI
-open LabeledRuntimeAPI
+open Comparse
+open DY.Core
+open DY.Lib
 open MLS.Crypto
 open MLS.TreeSync.NetworkTypes
 open MLS.Symbolic
-open MLS.Symbolic.Session
-open MLS.Symbolic.MapSession
 open MLS.TreeSync.Symbolic.LeafNodeSignature
 open MLS.TreeSync.Symbolic.AuthServiceCache
 open MLS.TreeSync.Symbolic.API.Sessions
@@ -18,130 +16,97 @@ open MLS.TreeSync.Symbolic.API.KeyPackageManager
 
 (*** Predicate definition ***)
 
-val treesync_key_usages: key_usages
-let treesync_key_usages = {
-  dh_shared_secret_usage = (fun _ _ _ -> None);
-  dh_unknown_peer_usage = (fun _ _ -> None);
-  dh_usage_commutes_lemma = (fun () -> ());
-  dh_unknown_peer_usage_lemma = (fun () -> ());
-  kdf_extend_label = (fun _ _ _ _ _ -> None);
-  kdf_extract_usage = (fun _ _ _ -> None);
-  kdf_expand_usage = (fun _ _ _ -> None);
-}
+instance treesync_crypto_usages: crypto_usages =
+  default_crypto_usages
 
-val can_sign_list: treekem_types dy_bytes -> list (valid_label & sign_pred)
-let can_sign_list tkt = [
-  (leaf_node_label, leaf_node_spred treesync_key_usages tkt);
+val all_sign_preds: treekem_types dy_bytes -> list (valid_label & mls_sign_pred)
+let all_sign_preds tkt = [
+  leaf_node_tbs_tag_and_invariant tkt;
 ]
 
-val treesync_usage_preds: treekem_types dy_bytes -> usage_preds
-let treesync_usage_preds tkt = {
-  can_pke_encrypt = (fun _ _ _ _ -> False);
-  can_aead_encrypt = (fun _ _ _ _ _ -> False);
-  can_sign = mk_can_sign (can_sign_list tkt);
-  can_mac = (fun _ _ _ _ -> False);
-}
-
-val treesync_global_usage: treekem_types dy_bytes -> global_usage
-let treesync_global_usage tkt = {
-  usage_preds = treesync_usage_preds tkt;
-  key_usages = treesync_key_usages;
-}
-
-val session_pred_list: tkt:treekem_types dy_bytes -> list (string & session_pred)
-let session_pred_list tkt = [
-  (as_cache_label, map_session_invariant as_cache_types as_cache_pred);
-  (group_manager_label, map_session_invariant group_manager_types group_manager_pred);
-  (key_package_manager_label, map_session_invariant (key_package_manager_types tkt) (key_package_manager_pred tkt));
-  (treesync_public_state_label, treesync_public_state_pred tkt);
-  (treesync_private_state_label, treesync_private_state_pred);
-]
-
-val treesync_trace_preds: tkt:treekem_types dy_bytes -> trace_preds (treesync_global_usage tkt)
-let treesync_trace_preds tkt = {
-  can_trigger_event = (fun time prin e -> True);
-  session_st_inv = mk_global_session_pred (session_pred_list tkt) (treesync_global_usage tkt);
-  session_st_inv_lemma = (fun time prin si vi st -> (
-    FStar.Classical.move_requires (mk_global_session_pred_is_msg (session_pred_list tkt) (treesync_global_usage tkt) time prin si vi) st
-  ));
-  session_st_inv_later = (fun time0 time1 prin si vi st ->
-    FStar.Classical.move_requires (mk_global_session_pred_later (session_pred_list tkt) (treesync_global_usage tkt) time0 time1 prin si vi) st
+val treesync_crypto_predicates: treekem_types dy_bytes -> crypto_predicates treesync_crypto_usages
+let treesync_crypto_predicates tkt = {
+  default_crypto_predicates treesync_crypto_usages with
+  sign_pred = mk_sign_pred (all_sign_preds tkt);
+  sign_pred_later = (fun tr1 tr2 vk msg ->
+    mk_sign_pred_later (all_sign_preds tkt) tr1 tr2 vk msg
   );
 }
 
-val treesync_preds: treekem_types dy_bytes -> preds
-let treesync_preds tkt = {
-  global_usage = treesync_global_usage tkt;
-  trace_preds = treesync_trace_preds tkt;
+instance treesync_crypto_invariants (tkt:treekem_types dy_bytes): crypto_invariants = {
+  usages = treesync_crypto_usages;
+  preds = treesync_crypto_predicates tkt;
+}
+
+val all_state_predicates: tkt:treekem_types dy_bytes -> list (string & local_bytes_state_predicate)
+let all_state_predicates tkt = [
+  as_cache_tag_and_invariant;
+  group_manager_tag_and_invariant;
+  key_package_manager_tag_and_invariant tkt;
+  treesync_public_state_tag_and_invariant tkt;
+  treesync_private_state_tag_and_invariant;
+]
+
+val treesync_trace_invariants: tkt:treekem_types dy_bytes -> trace_invariants (treesync_crypto_invariants tkt)
+let treesync_trace_invariants tkt = {
+  state_pred = mk_state_predicate (treesync_crypto_invariants tkt) (all_state_predicates tkt);
+  event_pred = mk_event_pred [];
+}
+
+val treesync_protocol_invariants: treekem_types dy_bytes -> protocol_invariants
+let treesync_protocol_invariants tkt = {
+  crypto_invs = treesync_crypto_invariants tkt;
+  trace_invs = treesync_trace_invariants tkt;
 }
 
 (*** Proofs ***)
 
-// This tactic is useful because `assert_norm` gets completely lost and eat all the RAM
-inline_for_extraction noextract
-val sign_memP_tactic: unit -> Tac unit
-let sign_memP_tactic () =
-  norm [delta_only [`%List.Tot.Base.memP; `%can_sign_list]; iota; zeta]
+val all_sign_preds_has_all_sign_preds: tkt:treekem_types dy_bytes -> Lemma (norm [delta_only [`%all_sign_preds; `%for_allP]; iota; zeta] (for_allP (has_sign_pred (treesync_crypto_invariants tkt)) (all_sign_preds tkt)))
+let all_sign_preds_has_all_sign_preds tkt =
+  assert_norm(List.Tot.no_repeats_p (List.Tot.map fst (all_sign_preds tkt)));
+  mk_sign_pred_correct (treesync_crypto_invariants tkt) (all_sign_preds tkt);
+  norm_spec [delta_only [`%all_sign_preds; `%for_allP]; iota; zeta] (for_allP (has_sign_pred (treesync_crypto_invariants tkt)) (all_sign_preds tkt));
+  let dumb_lemma (x:prop) (y:prop): Lemma (requires x /\ x == y) (ensures y) = () in
+  dumb_lemma (for_allP (has_sign_pred (treesync_crypto_invariants tkt)) (all_sign_preds tkt)) (norm [delta_only [`%all_sign_preds; `%for_allP]; iota; zeta] (for_allP (has_sign_pred (treesync_crypto_invariants tkt)) (all_sign_preds tkt)))
 
 val treesync_global_usage_has_leaf_node_tbs_invariant: tkt:treekem_types dy_bytes -> Lemma
-  (has_leaf_node_tbs_invariant tkt (treesync_global_usage tkt))
-  [SMTPat (has_leaf_node_tbs_invariant tkt (treesync_global_usage tkt))]
+  (has_leaf_node_tbs_invariant tkt (treesync_crypto_invariants tkt))
+  [SMTPat (has_leaf_node_tbs_invariant tkt (treesync_crypto_invariants tkt))]
 let treesync_global_usage_has_leaf_node_tbs_invariant tkt =
-  assert_norm(List.Tot.no_repeats_p (List.Tot.map fst (can_sign_list tkt)));
-  assert(List.Tot.memP (leaf_node_label, (leaf_node_spred treesync_key_usages tkt)) (can_sign_list tkt)) by (sign_memP_tactic());
-  mk_can_sign_correct (treesync_global_usage tkt) (can_sign_list tkt) leaf_node_label (leaf_node_spred treesync_key_usages tkt)
+  all_sign_preds_has_all_sign_preds tkt
 
-inline_for_extraction noextract
-val session_memP_tactic: unit -> Tac unit
-let session_memP_tactic () =
-  norm [delta_only [`%List.Tot.Base.memP; `%session_pred_list]; iota; zeta]
+val all_state_predicates_has_all_state_predicates: tkt:treekem_types dy_bytes -> Lemma (norm [delta_only [`%all_state_predicates; `%for_allP]; iota; zeta] (for_allP (has_local_bytes_state_predicate (treesync_protocol_invariants tkt)) (all_state_predicates tkt)))
+let all_state_predicates_has_all_state_predicates tkt =
+  assert_norm(List.Tot.no_repeats_p (List.Tot.map fst (all_state_predicates tkt)));
+  mk_global_local_bytes_state_predicate_correct (treesync_protocol_invariants tkt) (all_state_predicates tkt);
+  norm_spec [delta_only [`%all_state_predicates; `%for_allP]; iota; zeta] (for_allP (has_local_bytes_state_predicate (treesync_protocol_invariants tkt)) (all_state_predicates tkt))
 
-val treesync_preds_has_as_cache_invariant: tkt:treekem_types dy_bytes -> Lemma
-  (has_as_cache_invariant (treesync_preds tkt))
-  [SMTPat (has_as_cache_invariant (treesync_preds tkt))]
-let treesync_preds_has_as_cache_invariant tkt =
-  let lab = as_cache_label in
-  let spred = (map_session_invariant as_cache_types as_cache_pred) in
-  assert_norm(List.Tot.no_repeats_p (List.Tot.map fst (session_pred_list tkt)));
-  assert(List.Tot.memP (lab, spred) (session_pred_list tkt)) by (session_memP_tactic());
-  mk_global_session_pred_correct (treesync_preds tkt) (session_pred_list tkt) lab spred
+val treesync_protocol_invariants_has_as_cache_invariant: tkt:treekem_types dy_bytes -> Lemma
+  (has_as_cache_invariant (treesync_protocol_invariants tkt))
+  [SMTPat (has_as_cache_invariant (treesync_protocol_invariants tkt))]
+let treesync_protocol_invariants_has_as_cache_invariant tkt =
+  all_state_predicates_has_all_state_predicates tkt
 
-val treesync_preds_has_group_manager_invariant: tkt:treekem_types dy_bytes -> Lemma
-  (has_group_manager_invariant (treesync_preds tkt))
-  [SMTPat (has_group_manager_invariant (treesync_preds tkt))]
-let treesync_preds_has_group_manager_invariant tkt =
-  let lab = group_manager_label in
-  let spred = (map_session_invariant group_manager_types group_manager_pred) in
-  assert_norm(List.Tot.no_repeats_p (List.Tot.map fst (session_pred_list tkt)));
-  assert(List.Tot.memP (lab, spred) (session_pred_list tkt)) by (session_memP_tactic());
-  mk_global_session_pred_correct (treesync_preds tkt) (session_pred_list tkt) lab spred
+val treesync_protocol_invariants_has_group_manager_invariant: tkt:treekem_types dy_bytes -> Lemma
+  (has_group_manager_invariant (treesync_protocol_invariants tkt))
+  [SMTPat (has_group_manager_invariant (treesync_protocol_invariants tkt))]
+let treesync_protocol_invariants_has_group_manager_invariant tkt =
+  all_state_predicates_has_all_state_predicates tkt
 
-val treesync_preds_has_key_package_manager_invariant: tkt:treekem_types dy_bytes -> Lemma
-  (has_key_package_manager_invariant tkt (treesync_preds tkt))
-  [SMTPat (has_key_package_manager_invariant tkt (treesync_preds tkt))]
-let treesync_preds_has_key_package_manager_invariant tkt =
-  let lab = key_package_manager_label in
-  let spred = (map_session_invariant (key_package_manager_types tkt) (key_package_manager_pred tkt)) in
-  assert_norm(List.Tot.no_repeats_p (List.Tot.map fst (session_pred_list tkt)));
-  assert(List.Tot.memP (lab, spred) (session_pred_list tkt)) by (session_memP_tactic());
-  mk_global_session_pred_correct (treesync_preds tkt) (session_pred_list tkt) lab spred
+val treesync_protocol_invariants_has_key_package_manager_invariant: tkt:treekem_types dy_bytes -> Lemma
+  (has_key_package_manager_invariant tkt (treesync_protocol_invariants tkt))
+  [SMTPat (has_key_package_manager_invariant tkt (treesync_protocol_invariants tkt))]
+let treesync_protocol_invariants_has_key_package_manager_invariant tkt =
+  all_state_predicates_has_all_state_predicates tkt
 
-val treesync_preds_has_treesync_public_state_invariant: tkt:treekem_types dy_bytes -> Lemma
-  (has_treesync_public_state_invariant tkt (treesync_preds tkt))
-  [SMTPat (has_treesync_public_state_invariant tkt (treesync_preds tkt))]
-let treesync_preds_has_treesync_public_state_invariant tkt =
-  let lab = treesync_public_state_label in
-  let spred = treesync_public_state_pred tkt in
-  assert_norm(List.Tot.no_repeats_p (List.Tot.map fst (session_pred_list tkt)));
-  assert(List.Tot.memP (lab, spred) (session_pred_list tkt)) by (session_memP_tactic());
-  mk_global_session_pred_correct (treesync_preds tkt) (session_pred_list tkt) lab spred
+val treesync_protocol_invariants_has_treesync_public_state_invariant: tkt:treekem_types dy_bytes -> Lemma
+  (has_treesync_public_state_invariant tkt (treesync_protocol_invariants tkt))
+  [SMTPat (has_treesync_public_state_invariant tkt (treesync_protocol_invariants tkt))]
+let treesync_protocol_invariants_has_treesync_public_state_invariant tkt =
+  all_state_predicates_has_all_state_predicates tkt
 
-val treesync_preds_has_treesync_private_state_invariant: tkt:treekem_types dy_bytes -> Lemma
-  (has_treesync_private_state_invariant (treesync_preds tkt))
-  [SMTPat (has_treesync_private_state_invariant (treesync_preds tkt))]
-let treesync_preds_has_treesync_private_state_invariant tkt =
-  let lab = treesync_private_state_label in
-  let spred = treesync_private_state_pred in
-  assert_norm(List.Tot.no_repeats_p (List.Tot.map fst (session_pred_list tkt)));
-  assert(List.Tot.memP (lab, spred) (session_pred_list tkt)) by (session_memP_tactic());
-  mk_global_session_pred_correct (treesync_preds tkt) (session_pred_list tkt) lab spred
+val treesync_protocol_invariants_has_treesync_private_state_invariant: tkt:treekem_types dy_bytes -> Lemma
+  (has_treesync_private_state_invariant (treesync_protocol_invariants tkt))
+  [SMTPat (has_treesync_private_state_invariant (treesync_protocol_invariants tkt))]
+let treesync_protocol_invariants_has_treesync_private_state_invariant tkt =
+  all_state_predicates_has_all_state_predicates tkt
