fstar/treesync/symbolic/MLS.TreeSync.Symbolic.API.IsWellFormedInvariant.fst
@@ -18,38 +18,38 @@ open MLS.Result
 #set-options "--fuel 1 --ifuel 1"
 
 val is_well_formed_finalize_create:
-  #bytes:Type0 -> {|crypto_bytes bytes|} -> #tkt:treekem_types bytes -> #asp:as_parameters bytes ->
+  #bytes:Type0 -> {|crypto_bytes bytes|} -> #tkt:treekem_types bytes -> #token_t:Type0 ->
   #group_id:mls_bytes bytes -> #ln:leaf_node_nt bytes tkt ->
   pre:bytes_compatible_pre bytes ->
-  pend:pending_create group_id ln -> token:token_for_create asp pend ->
+  pend:pending_create group_id ln -> token:token_t ->
   Lemma
   (requires is_well_formed _ pre ln)
   (ensures (
     let new_state = finalize_create pend token in
     is_well_formed _ pre (new_state.tree <: treesync _ _ _ _)
   ))
-let is_well_formed_finalize_create #bytes #cb #tkt #asp #group_id #ln pre pend token =
+let is_well_formed_finalize_create #bytes #cb #tkt #token_t #group_id #ln pre pend token =
   ()
 
 val is_well_formed_finalize_welcome:
-  #bytes:Type0 -> {|crypto_bytes bytes|} -> #tkt:treekem_types bytes -> #asp:as_parameters bytes -> #l:nat ->
+  #bytes:Type0 -> {|crypto_bytes bytes|} -> #tkt:treekem_types bytes -> #token_t:Type0 -> #l:nat ->
   #group_id:mls_bytes bytes -> #t:treesync bytes tkt l 0 ->
   pre:bytes_compatible_pre bytes ->
-  pend:pending_welcome group_id t -> tokens:tokens_for_welcome asp pend ->
+  pend:pending_welcome group_id t -> tokens:list (option token_t){List.Tot.length tokens == pow2 l} ->
   Lemma
   (requires is_well_formed _ pre t)
   (ensures (
     let new_state = finalize_welcome pend tokens in
     is_well_formed _ pre (new_state.tree <: treesync _ _ _ _)
   ))
-let is_well_formed_finalize_welcome #bytes #cb #tkt #asp #l #group_id #t pre pend tokens =
+let is_well_formed_finalize_welcome #bytes #cb #tkt #token_t #l #group_id #t pre pend tokens =
   ()
 
 val is_well_formed_finalize_add:
-  #bytes:Type0 -> {|crypto_bytes bytes|} -> #tkt:treekem_types bytes -> #asp:as_parameters bytes -> #group_id:mls_bytes bytes ->
-  #st:treesync_state bytes tkt asp group_id -> #ln:leaf_node_nt bytes tkt ->
+  #bytes:Type0 -> {|crypto_bytes bytes|} -> #tkt:treekem_types bytes -> #token_t:Type0 -> #group_id:mls_bytes bytes ->
+  #st:treesync_state bytes tkt token_t group_id -> #ln:leaf_node_nt bytes tkt ->
   pre:bytes_compatible_pre bytes ->
-  pend:pending_add st ln -> token:token_for_add pend ->
+  pend:pending_add st ln -> token:token_t ->
   Lemma
   (requires
     is_well_formed _ pre (st.tree <: treesync _ _ _ _) /\
@@ -60,7 +60,7 @@ val is_well_formed_finalize_add:
     let Success (new_state, _) = finalize_add pend token in
     is_well_formed _ pre (new_state.tree <: treesync _ _ _ _)
   ))
-let is_well_formed_finalize_add #bytes #cb #tkt #asp #group_id #st #ln pre pend token =
+let is_well_formed_finalize_add #bytes #cb #tkt #token_t #group_id #st #ln pre pend token =
   match find_empty_leaf st.tree with
   | Some li -> (
     is_well_formed_tree_add pre st.tree li ln
@@ -74,22 +74,22 @@ let is_well_formed_finalize_add #bytes #cb #tkt #asp #group_id #st #ln pre pend 
   )
 
 val is_well_formed_finalize_update:
-  #bytes:Type0 -> {|crypto_bytes bytes|} -> #tkt:treekem_types bytes -> #asp:as_parameters bytes -> #group_id:mls_bytes bytes ->
-  #st:treesync_state bytes tkt asp group_id -> #ln:leaf_node_nt bytes tkt -> #li:treesync_index st ->
+  #bytes:Type0 -> {|crypto_bytes bytes|} -> #tkt:treekem_types bytes -> #token_t:Type0 -> #group_id:mls_bytes bytes ->
+  #st:treesync_state bytes tkt token_t group_id -> #ln:leaf_node_nt bytes tkt -> #li:treesync_index st ->
   pre:bytes_compatible_pre bytes ->
-  pend:pending_update st ln li -> token:token_for_update pend ->
+  pend:pending_update st ln li -> token:token_t ->
   Lemma
   (requires is_well_formed _ pre (st.tree <: treesync _ _ _ _) /\ is_well_formed _ pre ln)
   (ensures (
     let new_state = finalize_update pend token in
     is_well_formed _ pre (new_state.tree <: treesync _ _ _ _)
   ))
-let is_well_formed_finalize_update #bytes #cb #tkt #asp #group_id #st #ln #li pre pend token =
+let is_well_formed_finalize_update #bytes #cb #tkt #token_t #group_id #st #ln #li pre pend token =
   is_well_formed_tree_update pre st.tree li ln
 
 val is_well_formed_fully_truncate_state:
-  #bytes:Type0 -> {|crypto_bytes bytes|} -> #tkt:treekem_types bytes -> #asp:as_parameters bytes -> #group_id:mls_bytes bytes ->
-  st:treesync_state bytes tkt asp group_id ->
+  #bytes:Type0 -> {|crypto_bytes bytes|} -> #tkt:treekem_types bytes -> #token_t:Type0 -> #group_id:mls_bytes bytes ->
+  st:treesync_state bytes tkt token_t group_id ->
   pre:bytes_compatible_pre bytes ->
   Lemma
   (requires is_well_formed _ pre (st.tree <: treesync _ _ _ _))
@@ -98,19 +98,18 @@ val is_well_formed_fully_truncate_state:
     is_well_formed _ pre (new_state.tree <: treesync _ _ _ _)
   ))
   (decreases st.levels)
-let rec is_well_formed_fully_truncate_state #bytes #cb #tkt #asp #group_id st pre =
+let rec is_well_formed_fully_truncate_state #bytes #cb #tkt #token_t #group_id st pre =
   if 1 <= st.levels && is_tree_empty (TNode?.right st.tree) then (
-    MLS.TreeSync.Invariants.AuthService.Proofs.all_credentials_ok_tree_truncate st.tree st.tokens;
     is_well_formed_fully_truncate_state ({
       levels = st.levels-1;
       tree = tree_truncate st.tree;
       tokens = as_truncate st.tokens;
-    } <: treesync_state bytes tkt asp group_id) pre
+    } <: treesync_state bytes tkt token_t group_id) pre
   ) else ()
 
 val is_well_formed_finalize_remove:
-  #bytes:Type0 -> {|crypto_bytes bytes|} -> #tkt:treekem_types bytes -> #asp:as_parameters bytes -> #group_id:mls_bytes bytes ->
-  #st:treesync_state bytes tkt asp group_id -> #li:treesync_index st ->
+  #bytes:Type0 -> {|crypto_bytes bytes|} -> #tkt:treekem_types bytes -> #token_t:Type0 -> #group_id:mls_bytes bytes ->
+  #st:treesync_state bytes tkt token_t group_id -> #li:treesync_index st ->
   pre:bytes_compatible_pre bytes ->
   pend:pending_remove st li ->
   Lemma
@@ -119,16 +118,15 @@ val is_well_formed_finalize_remove:
     let new_state = finalize_remove pend in
     is_well_formed _ pre (new_state.tree <: treesync _ _ _ _)
   ))
-let is_well_formed_finalize_remove #bytes #cb #tkt #asp #group_id #st #li pre pend =
-  MLS.TreeSync.Invariants.AuthService.Proofs.all_credentials_ok_tree_remove st.tree st.tokens li;
+let is_well_formed_finalize_remove #bytes #cb #tkt #token_t #group_id #st #li pre pend =
   is_well_formed_tree_remove pre st.tree li;
   is_well_formed_fully_truncate_state (state_update_tree st (tree_remove st.tree li) (as_remove st.tokens li)) pre
 
 val is_well_formed_finalize_commit:
-  #bytes:Type0 -> {|crypto_bytes bytes|} -> #tkt:treekem_types bytes -> #asp:as_parameters bytes -> #group_id:mls_bytes bytes ->
-  #st:treesync_state bytes tkt asp group_id -> #li:treesync_index st -> #p:pathsync bytes tkt st.levels 0 li ->
+  #bytes:Type0 -> {|crypto_bytes bytes|} -> #tkt:treekem_types bytes -> #token_t:Type0 -> #group_id:mls_bytes bytes ->
+  #st:treesync_state bytes tkt token_t group_id -> #li:treesync_index st -> #p:pathsync bytes tkt st.levels 0 li ->
   pre:bytes_compatible_pre bytes{pre_is_hash_compatible pre} ->
-  pend:pending_commit st p -> token:token_for_commit pend ->
+  pend:pending_commit st p -> token:token_t ->
   Lemma
   (requires
     is_well_formed _ pre (st.tree <: treesync _ _ _ _) /\
@@ -139,5 +137,5 @@ val is_well_formed_finalize_commit:
     let Success new_state = finalize_commit pend token in
     is_well_formed _ pre (new_state.tree <: treesync _ _ _ _)
   ))
-let is_well_formed_finalize_commit #bytes #cb #tkt #asp #group_id #st #li #p pre pend token =
+let is_well_formed_finalize_commit #bytes #cb #tkt #token_t #group_id #st #li #p pre pend token =
   is_well_formed_apply_path pre st.tree p
